RelationalAlgebra/FOL/Realize.lean
@@ -16,392 +16,92 @@ theorem Term.realizeSome.def (dbi) [folStruc dbi] (t : fol.Term (Attribute ⊕ (
   Term.realizeSome dbi t tup iv ↔ (t.realize (Sum.elim tup iv)).Dom := by rfl
 
 @[simp]
-theorem Term.realizeSome.tuple_restrict {dbi} [folStruc dbi] (t : fol.Term (Attribute ⊕ (Fin n))) {tup tup' : Tuple} {iv : Fin n →. Value} :
-  Term.realizeSome dbi t tup' iv → (h_sub : tup'.Dom ⊆ tup.Dom) → tup' = tup.restrict h_sub → Term.realizeSome dbi t tup iv := by
-    intro h_realize h_sub h_eq
-    simp_all only [«def»]
-    have ⟨t, ht⟩ := Term.cases t
-    subst ht
-    cases t with
-    | inl a => exact h_sub h_realize
-    | inr k => simp_all only [realize_var, Sum.elim_inr]
+theorem Term.RealizeSome.fromRelMap [struc : folStruc dbi] (i) {tMap : Fin (dbi.schema rn).card → fol.Term (Attribute ⊕ Fin n)} {tup : Tuple} {iv : Fin n →. Value}
+  (h_rel : (struc.RelMap (fol.Rel dbi.schema rn) (fun i ↦ realize (Sum.elim tup iv) (tMap i))))
+  : Term.realizeSome dbi (tMap i) tup iv := by
+      simp_all only [folStruc_apply_RelMap, realizeSome.def]
+      apply Part.dom_iff_mem.mpr
+      have ⟨a', ha'⟩ : ∃a', a' = ((dbi.schema rn).fromIndex i) := by simp
+      have ⟨t', ht'⟩ : ∃t', t' = (ArityToTuple fun i ↦ realize (Sum.elim tup iv) (tMap i)) := by simp
+      have t'_Dom : a' ∈ t'.Dom := by
+        simp [RelationInstance.validSchema (dbi.relations rn) t' (by simp_all only), ha']
+      use (t' a').get t'_Dom
+      subst ht' ha'
+      simp_all only [folStruc_apply_RelMap, arityToTuple_def]
+      apply Part.get_mem
 
-theorem Term.realizeSome.tuple_restrict2 {dbi} [folStruc dbi] (t : fol.Term (Attribute ⊕ (Fin n))) {tup : Tuple} {iv : Fin n →. Value} :
-  Term.realizeSome dbi t tup iv → (h : ↑t.varFinsetLeft ⊆ tup.Dom) → tup' = tup.restrict h → Term.realizeSome dbi t tup' iv := by
-    intro a h ht
-    simp_all only [«def»]
-    have ⟨t, ht⟩ := Term.cases t
-    subst ht
-    cases t with
-    | inl a => simp [PFun.restrict, Part.restrict]
-    | inr k => simp_all only [realize_var, Sum.elim_inr, varFinsetLeft.eq_2, implies_true]
+-- Formal realization definition
+def BoundedQuery.Realize (dbi) {n : ℕ} [folStruc dbi] (q : BoundedQuery n): Tuple → (Fin n →. Value) → Prop :=
+  q.toFormula.Realize
 
--- Formal realization definition, requires all terms to be 'some'
-def BoundedQuery.Realize (dbi) {n : ℕ} [folStruc dbi] : BoundedQuery n → Tuple → (Fin n →. Value) → Prop
-  | R dbs rn tMap,  tup, iv => (∀i, Term.realizeSome dbi (tMap i) tup iv) ∧ (R dbs rn tMap).toFormula.Realize tup iv
-  | tEq q t₁ t₂,    tup, iv => q.Realize dbi tup iv ∧ Term.realizeSome dbi t₁ tup iv ∧ Term.realizeSome dbi t₂ tup iv
-                                ∧ (BoundedFormula.equal t₁ t₂).Realize tup iv
-  | and q₁ q₂,      tup, iv => q₁.Realize dbi tup iv ∧ q₂.Realize dbi tup iv
-  | ex q,           tup, iv => ∃a, q.Realize dbi tup (Fin.snoc iv a)
+theorem BoundedQuery.Realize.def [folStruc dbi] {tup : Tuple} {iv : Fin n →. Value} {q : BoundedQuery n}
+  : q.Realize dbi tup iv ↔ q.toFormula.Realize tup iv := by rfl
 
 @[simp]
-theorem BoundedQuery.Realize.R_def [folStruc dbi] {n : ℕ} (tMap) {tup : Tuple} {iv : Fin n →. Value}
-  : (R dbs rn tMap).Realize dbi tup iv ↔ (∀i, Term.realizeSome dbi (tMap i) tup iv) ∧ (R dbs rn tMap).toFormula.Realize tup iv := by
-    rfl
-
-theorem BoundedQuery.Realize.all_i_R_def [folStruc dbi] {n : ℕ} (tMap) {tup : Tuple} {iv : Fin n →. Value}
-  : (R dbs rn tMap).Realize dbi tup iv → (∀i, ((tMap i).realize (Sum.elim tup iv)).Dom) := by
-    simp_all
-
-theorem BoundedQuery.Realize.all_att_R_def [folStruc dbi] {n : ℕ} (tMap) {tup : Tuple} {iv : Fin n →. Value}
-  : (R dbs rn tMap).Realize dbi tup iv → (∀a (ha : a ∈ dbs rn), ((tMap ((dbs rn).index ha)).realize (Sum.elim tup iv)).Dom) := by
-    simp_all
-
-theorem BoundedQuery.Realize.exists_att_R_def [folStruc dbi] {n : ℕ} (tMap) {tup : Tuple} {iv : Fin n →. Value} (h : dbs rn ≠ ∅)
-  : (R dbs rn tMap).Realize dbi tup iv → (∃t' : fol.Term (Attribute ⊕ (Fin n)), (t'.realize (Sum.elim tup iv)).Dom) := by
-    intro a
-    simp_all only [ne_eq, R_def, realizeSome.def, toFormula_rel, BoundedFormula.realize_rel]
-    obtain ⟨left, right⟩ := a
-    induction h' : (dbs rn).card with
-    | zero => simp_all only [Finset.card_eq_zero]
-    | succ k ih =>
-      use (tMap (Fin.cast h'.symm (Fin.ofNat' (k + 1) (k + 1))))
-      simp_all only
+theorem BoundedQuery.Realize.all_att_R_def [folStruc dbi] {tup : Tuple} {iv : Fin n →. Value}
+  (h_wt : (R dbs rn tMap).isWellTyped dbi.schema)
+  (h_rel : (R dbs rn tMap).Realize dbi tup iv) (ha : a ∈ dbs rn) :
+    Term.realizeSome dbi (tMap ((dbs rn).index ha)) tup iv := by
+      simp_all
+      subst h_wt
+      exact Term.RealizeSome.fromRelMap ?_ h_rel
 
 @[simp]
-theorem BoundedQuery.Realize.exists_tuple_R_def [folStruc dbi] {n : ℕ} (tMap) {tup : Tuple} {iv : Fin n →. Value}
-  : (R dbi.schema rn tMap).Realize dbi tup iv → (∃t' ∈ (dbi.relations rn).tuples, ∀i, (tMap i).realize (Sum.elim tup iv) = t' ((dbi.schema rn).fromIndex i)) := by
-    intro a
-    simp_all only [R_def, realizeSome.def, toFormula_rel, BoundedFormula.realize_rel, folStruc_apply_RelMap]
-    obtain ⟨left, right⟩ := a
+theorem BoundedQuery.Realize.exists_t_R_def [folStruc dbi] {tup : Tuple} {iv : Fin n →. Value}
+  (h : dbs rn ≠ ∅) (h_wt : (R dbs rn tMap).isWellTyped dbi.schema)
+  (h_rel : (R dbs rn tMap).Realize dbi tup iv) :
+    (∃t : fol.Term (Attribute ⊕ (Fin n)), Term.realizeSome dbi t tup iv) := by
+      simp_all only [ne_eq, isWellTyped.R_def, «def», toFormula_rel, BoundedFormula.realize_rel,
+        realizeSome.def]
+      induction h' : (dbs rn).card with
+      | zero => simp_all only [Finset.card_eq_zero]
+      | succ k ih =>
+        use (tMap (Fin.cast h'.symm (Fin.ofNat' (k + 1) (k + 1))))
+        subst h_wt
+        exact Term.RealizeSome.fromRelMap ?_ h_rel
+
+@[simp]
+theorem BoundedQuery.Realize.exists_tuple_R_def [folStruc dbi] {tup : Tuple} {iv : Fin n →. Value}
+  (h_rel : (R dbi.schema rn tMap).Realize dbi tup iv)
+  : (∃t' ∈ (dbi.relations rn).tuples, ∀i, (tMap i).realize (Sum.elim tup iv) = t' ((dbi.schema rn).fromIndex i)) := by
+    simp_all only [«def», toFormula_rel, BoundedFormula.realize_rel, folStruc_apply_RelMap]
     use (ArityToTuple fun i ↦ realize (Sum.elim tup iv) (tMap i))
     simp_all only [true_and]
     intro i
     simp_all only [RelationSchema.fromIndex_mem, arityToTuple_def, and_self]
 
-@[simp]
-theorem BoundedQuery.Realize.tEq_def [folStruc dbi] {n : ℕ} (q : BoundedQuery n) (t₁ t₂ : fol.Term (Attribute ⊕ Fin n)) {tup : Tuple} {iv : Fin n →. Value}
-  : (tEq q t₁ t₂).Realize dbi tup iv ↔ (q.Realize dbi tup iv ∧ Term.realizeSome dbi t₁ tup iv ∧ Term.realizeSome dbi t₂ tup iv ∧ (BoundedFormula.equal t₁ t₂).Realize tup iv) := by
-    rfl
-
-@[simp]
-theorem BoundedQuery.Realize.and_def [folStruc dbi] {n : ℕ} (q₁ q₂ : BoundedQuery n) {t : Tuple} {iv : Fin n →. Value}
-  : (and q₁ q₂).Realize dbi t iv ↔ q₁.Realize dbi t iv ∧ q₂.Realize dbi t iv := by
-    rfl
-
-@[simp]
-theorem BoundedQuery.Realize.ex_def [folStruc dbi] {n : ℕ} (q : BoundedQuery (n + 1)) {t: Tuple} {iv : Fin n →. Value}
-  : (ex q).Realize dbi t iv ↔ ∃a, q.Realize dbi t (Fin.snoc iv a) := by
-    rfl
 
 @[simp]
 theorem BoundedQuery.Realize.exs_def [folStruc dbi] {n : ℕ} (q : BoundedQuery n) {t: Tuple}
   : (exs q).Realize dbi t (default : Fin 0 →. Value) ↔ ∃iv : Fin n →. Value, q.Realize dbi t iv := by
-    induction' n with n ih
-    · simp
-      apply Iff.intro
-      · intro a
-        use default
-      · intro a
-        obtain ⟨w, h⟩ := a
-        have hw : w = default := by
-          ext a v
-          exact Fin.elim0 a
-        simp_all only
-    · simp only [BoundedQuery.exs, ih, BoundedQuery.Realize.ex_def]
-      constructor
-      ·
-        intro a
-        obtain ⟨w, h⟩ := a
-        obtain ⟨w_1, h⟩ := h
-        apply Exists.intro
-        · exact h
-      · intro a
-        obtain ⟨w, h_1⟩ := a
-        use Fin.init w
-        use (w (Fin.last n))
-        simp_all only [Part.some_get, Fin.snoc_init_self, and_true]
+    simp_all only [«def», toFormula_exs, Formula.boundedFormula_realize_eq_realize]
+    exact BoundedFormula.realize_exs
 
 @[simp]
 theorem BoundedQuery.Realize.schema_sub_Dom [folStruc dbi] {n : ℕ} {q : BoundedQuery n} {t : Tuple} {iv : Fin n →. Value}
-  : q.Realize dbi t iv → ∀a ∈ q.schema, (t a).Dom := by
+  (h_wt : q.isWellTyped dbi.schema) (h_rel : q.Realize dbi t iv)
+  : ∀a ∈ q.schema, (t a).Dom := by
     induction q with
     | R dbs rn vs =>
-      intro a_1 a_2 a_3
-      simp_all only [R_def, realizeSome.def, toFormula_rel, BoundedFormula.realize_rel, schema.R_def, Set.mem_toFinset,
-        Set.mem_setOf_eq]
-      obtain ⟨left, right⟩ := a_1
-      obtain ⟨w, h⟩ := a_3
+      intro a_1 a_2
+      simp_all only [isWellTyped.R_def, «def», toFormula_rel, BoundedFormula.realize_rel,
+        schema.R_def, Set.mem_toFinset, Set.mem_setOf_eq]
+      obtain ⟨w, h⟩ := a_2
       have z := Term.cases (vs w)
       simp_all only [Sum.exists]
       cases z with
       | inl h_1 =>
         obtain ⟨w_1, h_1⟩ := h_1
-        simp_all only [varFinsetLeft.eq_1, Finset.mem_singleton]
+        simp_all only [isWellTyped.R_def, varFinsetLeft.eq_1, Finset.mem_singleton]
         subst h
-        have z' := left w
-        simp_all only [realize_var, Sum.elim_inl]
+        subst h_wt
+        have := Term.RealizeSome.fromRelMap w h_rel
+        simp_all only [isWellTyped.R_def, realizeSome.def, realize_var, Sum.elim_inl]
       | inr h_2 =>
         obtain ⟨w_1, h_1⟩ := h_2
         simp_all only [varFinsetLeft.eq_2, Finset.not_mem_empty]
 
-    | _ => aesop
-
-@[simp]
-theorem Relmap.tuple_restrict [folStruc : folStruc dbi] {t t' : Tuple} {tMap : Fin (dbi.schema rn).card → fol.Term (Attribute ⊕ (Fin n))}:
-  folStruc.RelMap (fol.Rel dbi.schema rn) (fun i ↦ realize (Sum.elim t' iv) (tMap i)) →
-  (h : t'.Dom ⊆ t.Dom) → t' = t.restrict h →
-  (∀ (i : Fin (Finset.card (dbi.schema rn))), (realize (Sum.elim (PFun.restrict t h) iv) (tMap i)).Dom) →
-    folStruc.RelMap (fol.Rel dbi.schema rn) (fun i ↦ realize (Sum.elim t iv) (tMap i)) := by
-      intro ht h ht' hdom
-      have z : (ArityToTuple fun i ↦ realize (Sum.elim (t.restrict h) iv) (tMap i)) = (ArityToTuple fun i ↦ realize (Sum.elim t iv) (tMap i)) := by
-        ext a v
-        apply Iff.intro
-        · intro a_1
-          unfold ArityToTuple at *
-          simp_all only [PFun.dom_mk, DatabaseInstance.validSchema_def]
-          split
-          next h_1 =>
-            simp_all only [↓reduceDIte, Part.dom_iff_mem]
-            have ⟨k, hk⟩ := Term.cases (tMap (RelationSchema.index h_1))
-            rw [hk]
-            simp_all only [realize_var]
-            cases k with
-            | inl val => simp_all only [Sum.elim_inl, PFun.mem_restrict, Finset.mem_coe]
-            | inr val_1 => simp_all only [Sum.elim_inr]
-          next h_1 => simp_all only [↓reduceDIte, Part.not_mem_none]
-        · intro a_1
-          unfold ArityToTuple at *
-          simp_all only [PFun.dom_mk, DatabaseInstance.validSchema_def]
-          split
-          next h_1 =>
-            simp_all only [↓reduceDIte]
-            have ⟨k, hk⟩ := Term.cases (tMap (RelationSchema.index h_1))
-            have z := hdom (RelationSchema.index h_1)
-            rw [hk]
-            simp_all only [realize_var]
-            cases k with
-            | inl val =>
-              simp [Part.dom_iff_mem] at z a_1
-              simp [a_1, z]
-            | inr val_1 => simp_all only [Sum.elim_inr]
-          next h_1 => simp_all only [↓reduceDIte, Part.not_mem_none]
-      simp_all only [folStruc_apply_RelMap]
-
-@[simp]
-theorem BoundedQuery.Realize.tuple_restrict [folStruc dbi] {n : ℕ} {q : BoundedQuery n} {t : Tuple} {iv : Fin n →. Value} (h_wt : q.isWellTyped dbi.schema)
-  : q.Realize dbi t' iv → (h : t'.Dom ⊆ t.Dom) →  t' = t.restrict h → q.Realize dbi t iv := by
-    intro a h a_1
-    induction q with
-    | R dbs rn tMap =>
-      simp_all only [R_def, realizeSome.def, toFormula_rel, BoundedFormula.realize_rel]
-      obtain ⟨left, right⟩ := a
-      apply And.intro
-      · intro i
-        exact Term.realizeSome.tuple_restrict (tMap i) (left i) h rfl
-      · simp_all
-        subst h_wt
-        exact Relmap.tuple_restrict right h rfl left
-
-    | tEq sq t₁ t₂ ih  =>
-      simp_all only [tEq_def, true_and]
-      obtain ⟨left, right⟩ := a
-      obtain ⟨left_1, right⟩ := right
-      obtain ⟨left_2, right⟩ := right
-      apply And.intro
-      . exact ih h_wt.1 left
-      . apply And.intro
-        · exact Term.realizeSome.tuple_restrict t₁ left_1 h rfl
-        · apply And.intro
-          · exact Term.realizeSome.tuple_restrict t₂ left_2 h rfl
-          · simp_all [BoundedFormula.Realize]
-            obtain ⟨left_1, right_1⟩ := h_wt
-            obtain ⟨left_3, right_1⟩ := right_1
-            have ⟨t₁, ht₁⟩ := Term.cases t₁
-            have ⟨t₂, ht₂⟩ := Term.cases t₂
-            simp_all [ht₁, ht₂]
-            cases t₁ with
-            | inl att₁ =>
-              simp_all
-              cases t₂ with
-              | inl att₂ =>
-                by_cases hd₁ : (t' att₁).Dom
-                . by_cases hd₂ : (t' att₂).Dom
-                  . simp [Part.ext_iff] at right ⊢
-                    simp [Part.dom_iff_mem] at hd₁ hd₂
-                    intro v
-                    apply Iff.intro
-                    . intro hv
-                      exact ((right v).mp (And.intro hd₁ hv)).2
-                    . intro hv
-                      exact ((right v).mpr (And.intro hd₂ hv)).2
-                  . simp_all
-                . simp_all
-              | inr fin₂ =>
-                by_cases (t' att₁).Dom
-                . simp_all
-                  rw [← right]
-                  ext v
-                  simp [PFun.mem_restrict]
-                  intro a
-                  subst ht₁ ht₂
-                  simp_all only
-                  exact Part.dom_iff_mem.mp left_2
-                . simp_all
-            | inr fin₁ =>
-              cases t₂ with
-              | inl att₂ =>
-                by_cases (t' att₂).Dom
-                . simp_all
-                  ext v
-                  simp [PFun.mem_restrict]
-                  intro a
-                  subst ht₁ ht₂
-                  simp_all only
-                  exact Part.dom_iff_mem.mp left_2
-                . simp_all
-              | inr fin₂ =>
-                simp_all
-
-    | ex q ih =>
-      simp at a ⊢ h_wt
-      have ⟨w, hw⟩ := a
-      use w
-      simp_all only [forall_const]
-
-    | _ => aesop
-
-@[simp]
-theorem Relmap.tuple_restrict2 [folStruc : folStruc dbi] {t : Tuple} (h : ↑((BoundedQuery.R dbi.schema rn tMap).schema) ⊆ t.Dom) :
-  folStruc.RelMap (fol.Rel dbi.schema rn) (fun i ↦ realize (Sum.elim t iv) (tMap i)) →
-    folStruc.RelMap (fol.Rel dbi.schema rn) (fun i ↦ realize (Sum.elim (PFun.restrict t h) iv) (tMap i)) := by
-      intro ht
-      have z : (ArityToTuple fun i ↦ realize (Sum.elim (t.restrict h) iv) (tMap i)) = (ArityToTuple fun i ↦ realize (Sum.elim t iv) (tMap i)) := by
-        ext a v
-        apply Iff.intro
-        · intro a_1
-          unfold ArityToTuple at *
-          simp_all only [PFun.dom_mk, DatabaseInstance.validSchema_def]
-          split
-          next h_1 =>
-            simp_all only [↓reduceDIte, Part.dom_iff_mem]
-            have ⟨k, hk⟩ := Term.cases (tMap (RelationSchema.index h_1))
-            rw [hk]
-            simp_all only [realize_var]
-            cases k with
-            | inl val => simp_all only [Sum.elim_inl, PFun.mem_restrict, Finset.mem_coe]
-            | inr val_1 => simp_all only [Sum.elim_inr]
-          next h_1 => simp_all only [↓reduceDIte, Part.not_mem_none]
-        · intro a_1
-          simp_all
-          have arityDom := RelationInstance.validSchema.def ht
-          unfold ArityToTuple at *
-          simp_all only [PFun.dom_mk, DatabaseInstance.validSchema_def]
-          split
-          next h_1 =>
-            simp_all only [↓reduceDIte]
-            have ⟨k, hk⟩ := Term.cases (tMap (RelationSchema.index h_1))
-            rw [hk]
-            simp_all only [realize_var]
-            cases k with
-            | inl
-              val =>
-              simp_all only [Sum.elim_inl, PFun.mem_restrict, BoundedQuery.schema.R_def, Set.coe_toFinset,
-                Set.mem_setOf_eq, and_true]
-              simp_all only [BoundedQuery.schema.R_def, Set.coe_toFinset]
-              use RelationSchema.index h_1
-              unfold varFinsetLeft
-              split
-              . simp_all only [var.injEq, Sum.inl.injEq, Finset.mem_singleton]
-              . simp_all only [var.injEq, reduceCtorEq]
-              . simp_all [emptyStructure]
-            | inr val_1 => simp_all only [Sum.elim_inr]
-          next h_1 => simp_all only [↓reduceDIte, Part.not_mem_none]
-      simp_all only [folStruc_apply_RelMap]
-
-@[simp]
-theorem BoundedQuery.Realize.tuple_restrict2 [folStruc dbi] {n : ℕ} {q : BoundedQuery n} {t : Tuple} {iv : Fin n →. Value} (h_wt : q.isWellTyped dbi.schema)
-  : (h : ↑q.schema ⊆ t.Dom) → q.Realize dbi t iv → q.Realize dbi (t.restrict h) iv := by
-    intro h h_rel
-    induction q with
-    | R dbs rn tMap =>
-      simp_all only [isWellTyped.R_def, R_def, toFormula_rel, BoundedFormula.realize_rel]
-      obtain ⟨left, right⟩ := h_rel
-      apply And.intro
-      · intro i
-        have z : ↑(tMap i).varFinsetLeft ⊆ t.Dom := by rw [@Set.subset_def] at ⊢ h; aesop
-        have z' := Term.realizeSome.tuple_restrict2 (tMap i) (left i) z (rfl)
-        have hz' : ↑(tMap i).varFinsetLeft ⊆ ↑(R dbs rn tMap).schema := by simp [Set.subset_def]; intro x hx; use i
-        exact realizeSome.tuple_restrict (tMap i) z' hz' rfl
-      · subst h_wt
-        simp_all [Relmap.tuple_restrict2 h right]
-
-
-    | tEq sq t₁ t₂ ih  =>
-      simp_all only [isWellTyped.tEq_def, tEq_def, forall_const]
-      obtain ⟨left, right⟩ := h_rel
-      obtain ⟨left_1, right⟩ := right
-      obtain ⟨left_2, right⟩ := right
-      have ⟨t₁, ht₁⟩ := Term.cases t₁
-      subst ht₁
-      have ⟨t₂, ht₂⟩ := Term.cases t₂
-      subst ht₂
-      simp_all only [realizeSome.def, realize_var, true_and]
-      obtain ⟨left_3, right_1⟩ := h_wt
-      obtain ⟨left_4, right_1⟩ := right_1
-      cases t₁ with
-      | inl val =>
-        cases t₂ with
-        | inl val_1 =>
-          simp_all only [Sum.elim_inl, hasSafeTerm_mem_schema]
-          apply And.intro
-          · exact left_4
-          · apply And.intro
-            · exact right_1
-            · ext a : 1
-              simp_all only [Part.dom_iff_mem, BoundedFormula.Realize, realize_var, Sum.elim_inl,
-                schema, PFun.mem_restrict, Finset.mem_coe, true_and]
-        | inr val_2 =>
-          simp_all only [Sum.elim_inl, hasSafeTerm_mem_schema, Sum.elim_inr, true_and]
-          apply And.intro
-          · exact left_4
-          · simp_all only [BoundedFormula.Realize, realize_var, Sum.elim_inl, Sum.elim_inr]
-            ext a : 1
-            simp_all only [PFun.mem_restrict, schema.tEq_def, Finset.mem_coe, true_and]
-      | inr val_1 =>
-        cases t₂ with
-        | inl val =>
-          simp_all only [Sum.elim_inr, Sum.elim_inl, hasSafeTerm_mem_schema, true_and]
-          apply And.intro
-          · exact right_1
-          · ext a : 1
-            simp_all only [Part.dom_iff_mem, BoundedFormula.Realize, realize_var, Sum.elim_inr,
-              Sum.elim_inl, schema, PFun.mem_restrict, Finset.mem_coe, true_and]
-        | inr val_2 =>
-          simp_all only [Sum.elim_inr, true_and]
-          exact right
-
-    | and q₁ q₂ ih₁ ih₂ =>
-      simp_all only [isWellTyped.and_def, and_self, and_def, forall_const]
-      obtain ⟨left, right⟩ := h_wt
-      obtain ⟨left_1, right_1⟩ := h_rel
-      apply And.intro
-      · have h': ↑q₁.schema ⊆ t.Dom := by simp_all
-        have := ih₁ h' left_1
-        have h'' : ↑q₁.schema ⊆ ↑(q₁.and q₂).schema := by simp
-        exact tuple_restrict left (ih₁ h' left_1) h'' rfl
-      · have h': ↑q₂.schema ⊆ t.Dom := by simp_all
-        have := ih₂ h' right_1
-        have h'' : ↑q₂.schema ⊆ ↑(q₁.and q₂).schema := by simp
-        exact tuple_restrict right (ih₂ h' right_1) h'' rfl
-
-    | ex q ih =>
-      simp_all only [isWellTyped.ex_def, ex_def, Part.coe_some, forall_const]
-      obtain ⟨w, h_1⟩ := h_rel
-      apply Exists.intro
-      · apply @ih
-        simp_all only [schema.ex_def, forall_true_left]
-        apply h_1
+    | _ => simp_all [BoundedQuery.Realize.def]; aesop
 
 theorem BoundedQuery.Realize.mapTermRel_add_castLe {dbi} [struc : folStruc dbi] {k : ℕ}
     {ft : ∀ n, fol.Term (Attribute ⊕ (Fin n)) → fol.Term (Attribute ⊕ (Fin (k + n)))}
@@ -414,16 +114,13 @@ theorem BoundedQuery.Realize.mapTermRel_add_castLe {dbi} [struc : folStruc dbi] 
     (φ.mapTermRel ft fun _ => BoundedQuery.castLE (add_assoc _ _ _).symm.le).Realize dbi v' xs ↔
       φ.Realize dbi (v xs) (xs ∘ Fin.natAdd _) := by
         induction φ with
-        | R => simp [FOL.BoundedQuery.mapTermRel, h1]
+        | R => simp [FOL.BoundedQuery.mapTermRel, h1, BoundedQuery.Realize.def]
         | tEq q t₁ t₂ ih =>
           rename_i n'
-          simp [FOL.BoundedQuery.mapTermRel, h1, hv, ih]
-          intro a a_1 a_2
-          have ⟨t₁, ht₁⟩ := Term.cases t₁
-          have ⟨t₂, ht₂⟩ := Term.cases t₂
-          simp_all only [realize_var, BoundedFormula.Realize]
-        | and _ _ ih1 ih2 => simp [FOL.BoundedQuery.mapTermRel, ih1, ih2]
-        | ex _ ih => simp [FOL.BoundedQuery.mapTermRel, ih, hv]
+          simp [FOL.BoundedQuery.mapTermRel, h1, hv, ih, BoundedQuery.Realize.def]
+          simp_all only [«def», mapTermRel_formula, BoundedFormula.Realize, realize_var]
+        | and _ _ ih1 ih2 => simp_all [FOL.BoundedQuery.mapTermRel, ih1, ih2, BoundedQuery.Realize.def]
+        | ex _ ih => simp_all [FOL.BoundedQuery.mapTermRel, ih, hv, BoundedQuery.Realize.def]
 
 @[simp]
 theorem BoundedQuery.Realize.relabel_def {dbi} [folStruc dbi] {m n : ℕ} {φ : BoundedQuery n}  {g : Attribute → Attribute ⊕ (Fin m)} {t : Tuple}
@@ -433,25 +130,47 @@ theorem BoundedQuery.Realize.relabel_def {dbi} [folStruc dbi] {m n : ℕ} {φ : 
       apply BoundedQuery.Realize.mapTermRel_add_castLe <;> simp
 
 @[simp]
-theorem BoundedQuery.Realize.all_terms {dbi} [folStruc dbi] {n : ℕ} {φ : BoundedQuery n} {t : Tuple} {xs : Fin n →. Value} :
-  φ.Realize dbi t xs → ∀term, φ.hasSafeTerm term → (term.realize (Sum.elim t xs)).Dom := by
-    induction φ with
-    | ex q ih =>
-      intro a term a_1
-      simp_all only [ex_def, hasSafeTerm.ex_def]
-      obtain ⟨w, h⟩ := a
-      have z := ih h ((Term.relabel (Sum.map id (Fin.castLE (by simp))) term)) a_1
-      simp_all only [Part.dom_iff_mem, realize_relabel]
-      obtain ⟨z, hz⟩ := z
-      use z
-      have ⟨z', hz'⟩ := Term.cases term
-      subst hz'
-      cases z'
-      . simp_all
-      . simp_all [Fin.snoc]
-        exact hz
+theorem BoundedQuery.Realize.all_terms {dbi} [folStruc dbi] {n : ℕ} {φ : BoundedQuery n} {t : Tuple} {xs : Fin n →. Value}
+  (h_wt : φ.isWellTyped dbi.schema) (h_rel : φ.Realize dbi t xs) :
+    ∀term, φ.hasSafeTerm term → (term.realize (Sum.elim t xs)).Dom := by
+      induction φ with
+      | ex q ih =>
+        intro term a_1
+        simp only [«def», isWellTyped.ex_def, toFormula_ex, BoundedFormula.realize_ex,
+          Nat.succ_eq_add_one, hasSafeTerm.ex_def, forall_const, implies_true] at h_wt h_rel ⊢
+        obtain ⟨w, h⟩ := h_rel
+        have z := ih h_wt h ((Term.relabel (Sum.map id (Fin.castLE (by simp))) term)) a_1
+        simp_all only [Part.dom_iff_mem, realize_relabel]
+        obtain ⟨z, hz⟩ := z
+        use z
+        have ⟨z', hz'⟩ := Term.cases term
+        subst hz'
+        cases z'
+        . simp_all
+        . simp_all [Fin.snoc]
+          exact hz
 
-    | _ => aesop
+      | R dbs rn tMap =>
+        intro term a_1
+        simp_all only [isWellTyped.R_def, toFormula_rel, BoundedFormula.realize_rel,
+          hasSafeTerm.R_def]
+        obtain ⟨w, h⟩ := a_1
+        subst h
+        subst h_wt
+        exact Term.RealizeSome.fromRelMap w h_rel
+
+      | and q₁ q₂ ih₁ ih₂ =>
+        simp only [isWellTyped.and_def, «def», toFormula_and, BoundedFormula.realize_inf,
+          hasSafeTerm.and_def] at h_wt h_rel ⊢
+        intro term a
+        simp_all only [«def», forall_const]
+        obtain ⟨left, right⟩ := h_wt
+        obtain ⟨left_1, right_1⟩ := h_rel
+        cases a with
+        | inl h => simp_all only
+        | inr h_1 => simp_all only
+
+      | _ => simp_all [BoundedQuery.Realize.def]
 
 @[simp]
 theorem BoundedQuery.Realize.tuple_eq_ext {dbi} [folStruc dbi] {n : ℕ} {φ : BoundedQuery n} {t t' : Tuple} {xs : Fin n →. Value} :
@@ -473,16 +192,5 @@ nonrec def Query.RealizeDom (φ : Query) (dbi : DatabaseInstance) [folStruc dbi]
 theorem Query.RealizeDom.def [folStruc dbi] (φ : Query)
   : φ.RealizeDom dbi t ↔ BoundedQuery.Realize dbi φ t default ∧ t.Dom ⊆ φ.schema := by rfl
 
-theorem Query.RealizeDom.schema_sub_Dom [folStruc dbi] {q : FOL.Query} (h: q.RealizeDom dbi t) :
-  ↑q.schema ⊆ t.Dom := by simp_all; exact BoundedQuery.Realize.schema_sub_Dom h.1
-
-@[simp]
-theorem Query.RealizeDom.imp_Realize {t dbi} [folStruc dbi] (φ : Query) :
-    φ.RealizeDom dbi t → φ.Realize dbi t default := by
-      simp_all
-
-@[simp]
-theorem Query.Realize.imp_RealizeDom_if_t_Dom_sub_schema {t dbi} [folStruc dbi]
-    (φ : Query) (h_dom_schema : t.Dom ⊆ ↑φ.schema) :
-    φ.Realize dbi t default → φ.RealizeDom dbi t := by
-      simp_all
+theorem Query.RealizeDom.schema_sub_Dom [folStruc dbi] {q : FOL.Query} (h_wt : q.isWellTyped dbi.schema) (h_rel : q.RealizeDom dbi t) :
+  ↑q.schema ⊆ t.Dom := by simp_all; exact BoundedQuery.Realize.schema_sub_Dom h_wt h_rel.1
