RelationalAlgebra/Equivalence/RAtoFOL/Relation.lean
@@ -5,34 +5,28 @@ variable {dbi rn} [struc : FOL.folStruc dbi]
 theorem ra_to_fol_evalT.R_def.mp :
     ∀t, (ra_to_fol_query (.R rn) dbi.schema).RealizeDom dbi t → t ∈ RA.Query.evaluateT dbi (.R rn) := by
       intro t
-      simp_all only [FOL.Query.RealizeDom.def, ra_to_fol_query.isWellTyped, ra_to_fol_query_schema,
-        ra_to_fol_query, Nat.add_zero, FOL.BoundedQuery.relabel.R_def, Function.comp_apply,
-        FOL.outVar.def, FirstOrder.Language.Term.relabel.eq_1, FOL.BoundedQuery.isWellTyped.R_def,
-        FOL.BoundedQuery.Realize.R_def, FOL.Term.realizeSome.def,
-        FirstOrder.Language.Term.realize_var, Sum.elim_inl, FOL.BoundedQuery.toFormula_rel,
-        FirstOrder.Language.BoundedFormula.realize_rel, FOL.folStruc_apply_RelMap,
-        FOL.BoundedQuery.schema.R_def, FirstOrder.Language.Term.varFinsetLeft.eq_1,
-        Finset.mem_singleton, RM.RelationSchema.Dom_sub_fromIndex, Finset.toFinset_coe,
-        RA.Query.evaluateT.R_def, and_imp]
-      intro a a_1 a_2
-      rw [FOL.ArityToTuple.def_fromIndex t] at a_1
+      simp_all only [ra_to_fol_query, FOL.Query.RealizeDom.def, FOL.BoundedQuery.Realize.def,
+        FOL.BoundedQuery.toFormula_rel, FirstOrder.Language.BoundedFormula.realize_rel,
+        Function.comp_apply, FOL.outVar.def, FirstOrder.Language.Term.realize_var, Sum.elim_inl,
+        FOL.folStruc_apply_RelMap, FOL.BoundedQuery.schema.R_def,
+        FirstOrder.Language.Term.varFinsetLeft.eq_1, Finset.mem_singleton,
+        RM.RelationSchema.Dom_sub_fromIndex, Finset.toFinset_coe, RA.Query.evaluateT.R_def, and_imp]
+      intro a a_1
+      rw [FOL.ArityToTuple.def_fromIndex t] at a
+      . exact a
       . exact a_1
-      . exact a_2
 
 theorem ra_to_fol_evalT.R_def.mpr (h : RA.Query.isWellTyped dbi.schema (.R rn)) :
   ∀t, t ∈ RA.Query.evaluateT dbi (.R rn) → (ra_to_fol_query (.R rn) dbi.schema).RealizeDom dbi t := by
     intro t h_RA_eval
-    apply
-      FOL.Query.Realize.imp_RealizeDom_if_t_Dom_sub_schema
-        (ra_to_fol_query (.R rn) dbi.schema)
-        (by simp_all [RA.Query.evaluate.validSchema (.R rn) h t h_RA_eval, ra_to_fol_query_schema])
+    apply And.intro ?_
+      (by simp_all [RA.Query.evaluate.validSchema (.R rn) h t h_RA_eval, ra_to_fol_query_schema])
 
     simp only [ra_to_fol_query]
     simp_all only [RA.Query.isWellTyped.R_def, RA.Query.evaluateT.R_def,
-      FOL.BoundedQuery.Realize.R_def, Function.comp_apply, FOL.outVar.def,
-      FOL.Term.realizeSome.def, FirstOrder.Language.Term.realize_var, Sum.elim_inl,
-      RM.RelationSchema.fromIndex_Dom, implies_true, FOL.BoundedQuery.toFormula_rel,
-      FirstOrder.Language.BoundedFormula.realize_rel, FOL.folStruc_apply_RelMap, true_and]
+      FOL.BoundedQuery.Realize.def, FOL.BoundedQuery.toFormula_rel,
+      FirstOrder.Language.BoundedFormula.realize_rel, Function.comp_apply, FOL.outVar.def,
+      FirstOrder.Language.Term.realize_var, Sum.elim_inl, FOL.folStruc_apply_RelMap]
 
     rw [FOL.ArityToTuple.def_fromIndex t]
     . exact h_RA_eval
