RelationalAlgebra/Equivalence/RAtoFOL/Rename.lean
@@ -25,10 +25,8 @@ theorem ra_to_fol_evalT.r_def.mpr (h : RA.Query.isWellTyped dbi.schema (.r f q))
   (ih : ∀t ∈ RA.Query.evaluateT dbi q, (ra_to_fol_query q dbi.schema).RealizeDom dbi t) :
     ∀t, t ∈ RA.Query.evaluateT dbi (.r f q) → (ra_to_fol_query (.r f q) dbi.schema).RealizeDom dbi t := by
       intro t h_RA_eval
-      apply
-        FOL.Query.Realize.imp_RealizeDom_if_t_Dom_sub_schema
-          (ra_to_fol_query (.r f q) dbi.schema)
-          (by simp_all [RA.Query.evaluate.validSchema (.r f q) h t h_RA_eval, ra_to_fol_query_schema])
+      apply And.intro ?_
+        (by simp_all [RA.Query.evaluate.validSchema (.r f q) h t h_RA_eval, ra_to_fol_query_schema])
 
       simp only [ra_to_fol_query]
       simp_all only [FOL.Query.RealizeDom.def, ra_to_fol_query.isWellTyped, ra_to_fol_query_schema,
