RelationalAlgebra/Equivalence/RAtoFOL/Selection.lean
@@ -6,37 +6,36 @@ theorem ra_to_fol_evalT.s_def.mp (h : RA.Query.isWellTyped dbi.schema (.s a b p 
   (ih: ∀t, (ra_to_fol_query q dbi.schema).RealizeDom dbi t → t ∈ RA.Query.evaluateT dbi q) :
     ∀t, (ra_to_fol_query (.s a b p q) dbi.schema).RealizeDom dbi t → t ∈ RA.Query.evaluateT dbi (.s a b p q) := by
       intro t
-      simp [RA.Query.isWellTyped.s_def, ra_to_fol_query, FOL.outVar.def,
-        FOL.Query.RealizeDom.def, FOL.BoundedQuery.Realize.tEq_def, FOL.Term.realizeSome.def,
-        FirstOrder.Language.Term.realize_var, Sum.elim_inl, FOL.BoundedQuery.schema.tEq_def,
+      simp only [RA.Query.isWellTyped.s_def, ra_to_fol_query, FOL.outVar.def,
+        FOL.Query.RealizeDom.def, FOL.BoundedQuery.Realize.def, FOL.BoundedQuery.toFormula_tEq,
+        FirstOrder.Language.BoundedFormula.realize_inf, FOL.BoundedQuery.schema.tEq_def,
         RA.Query.evaluateT.s_def, selectionT, ↓reduceIte, Set.mem_setOf_eq, and_imp] at ⊢ h
-      intro a_4 a_5 a_6 a_7 a_8
-      simp_all [ra_to_fol_query.isWellTyped, ra_to_fol_query_schema]
-      exact a_7
+      intro a_1 a_2 a_3
+      simp_all only [FOL.Query.RealizeDom.def, ra_to_fol_query.isWellTyped, and_imp]
+      obtain ⟨left, right⟩ := h
+      obtain ⟨left_1, right⟩ := right
+      apply And.intro
+      · apply ih
+        · exact a_1
+        · simp_all only [ra_to_fol_query.isWellTyped]
+      · exact a_2
 
 theorem ra_to_fol_evalT.s_def.mpr (h : RA.Query.isWellTyped dbi.schema (.s a b p q))
   (ih : ∀t ∈ RA.Query.evaluateT dbi q, (ra_to_fol_query q dbi.schema).RealizeDom dbi t) :
     ∀t, t ∈ RA.Query.evaluateT dbi (.s a b p q) → (ra_to_fol_query (.s a b p q) dbi.schema).RealizeDom dbi t := by
       intro t h_RA_eval
-      apply
-        FOL.Query.Realize.imp_RealizeDom_if_t_Dom_sub_schema
-          (ra_to_fol_query (.s a b p q) dbi.schema)
-          (by simp_all [RA.Query.evaluate.validSchema (.s a b p q) h t h_RA_eval, ra_to_fol_query_schema])
+      apply And.intro ?_
+        (by simp_all [RA.Query.evaluate.validSchema (.s a b p q) h t h_RA_eval, ra_to_fol_query_schema])
 
       simp only [ra_to_fol_query]
       simp_all only [RA.Query.isWellTyped.s_def, FOL.Query.RealizeDom.def,
-        ra_to_fol_query.isWellTyped, ra_to_fol_query_schema, forall_const, RA.Query.evaluateT.s_def,
-        selectionT, ne_eq, ite_true, Set.mem_setOf_eq, FOL.outVar.def,
-        FOL.BoundedQuery.Realize.tEq_def, FOL.Term.realizeSome.def,
-        FirstOrder.Language.Term.realize_var, Sum.elim_inl, and_self_left, true_and]
+        FOL.BoundedQuery.Realize.def, ra_to_fol_query_schema, RA.Query.evaluateT.s_def, selectionT,
+        ne_eq, ite_true, Set.mem_setOf_eq, FOL.outVar.def, FOL.BoundedQuery.toFormula_tEq,
+        FirstOrder.Language.BoundedFormula.realize_inf, true_and]
       obtain ⟨left, right⟩ := h
       obtain ⟨left_1, right_1⟩ := h_RA_eval
       obtain ⟨left_2, right⟩ := right
-      apply And.intro
-      · have z : ∀x, x ∈ q.schema dbi.schema ↔ (t x).Dom := by
-          simp [(RA.Query.evaluate dbi q left).validSchema t left_1, RA.Query.evaluate, Part.dom_iff_mem, ← PFun.mem_dom]
-        simp_all only
-      · exact right_1
+      exact right_1
 
 theorem ra_to_fol_evalT.s_def_eq (h : RA.Query.isWellTyped dbi.schema (.s a b p q))
   (ih: (ra_to_fol_query q dbi.schema).evaluateT dbi = RA.Query.evaluateT dbi q) :
