RelationalAlgebra/FOL/RealizeProperties.lean
@@ -1,0 +1,271 @@
+import RelationalAlgebra.FOL.Realize
+
+open FOL FirstOrder Language RM Term
+
+namespace FOL
+
+@[simp]
+theorem Term.realizeSome.tuple_restrict {dbi} [folStruc dbi] (t : fol.Term (Attribute ⊕ (Fin n))) {tup tup' : Tuple} {iv : Fin n →. Value} :
+  Term.realizeSome dbi t tup' iv → (h_sub : tup'.Dom ⊆ tup.Dom) → tup' = tup.restrict h_sub → Term.realizeSome dbi t tup iv := by
+    intro h_realize h_sub h_eq
+    simp_all only [«def»]
+    have ⟨t, ht⟩ := Term.cases t
+    subst ht
+    cases t with
+    | inl a => exact h_sub h_realize
+    | inr k => simp_all only [realize_var, Sum.elim_inr]
+
+theorem Term.realizeSome.tuple_restrict2 {dbi} [folStruc dbi] (t : fol.Term (Attribute ⊕ (Fin n))) {tup : Tuple} {iv : Fin n →. Value} :
+  Term.realizeSome dbi t tup iv → (h : ↑t.varFinsetLeft ⊆ tup.Dom) → tup' = tup.restrict h → Term.realizeSome dbi t tup' iv := by
+    intro a h ht
+    simp_all only [«def»]
+    have ⟨t, ht⟩ := Term.cases t
+    subst ht
+    cases t with
+    | inl a => simp [PFun.restrict, Part.restrict]
+    | inr k => simp_all only [realize_var, Sum.elim_inr, varFinsetLeft.eq_2, implies_true]
+
+
+@[simp]
+theorem Relmap.tuple_restrict [folStruc : folStruc dbi] {t t' : Tuple} {tMap : Fin (dbi.schema rn).card → fol.Term (Attribute ⊕ (Fin n))}:
+  folStruc.RelMap (fol.Rel dbi.schema rn) (fun i ↦ realize (Sum.elim t' iv) (tMap i)) →
+  (h : t'.Dom ⊆ t.Dom) → t' = t.restrict h →
+    folStruc.RelMap (fol.Rel dbi.schema rn) (fun i ↦ realize (Sum.elim t iv) (tMap i)) := by
+      intro ht h ht'
+      have z : (ArityToTuple fun i ↦ realize (Sum.elim (t.restrict h) iv) (tMap i)) = (ArityToTuple fun i ↦ realize (Sum.elim t iv) (tMap i)) := by
+        ext a v
+        apply Iff.intro
+        · intro a_1
+          unfold ArityToTuple at *
+          simp_all only [PFun.dom_mk, DatabaseInstance.validSchema_def]
+          split
+          next h_1 =>
+            simp_all only [↓reduceDIte, Part.dom_iff_mem]
+            have ⟨k, hk⟩ := Term.cases (tMap (RelationSchema.index h_1))
+            rw [hk]
+            simp_all only [realize_var]
+            cases k with
+            | inl val => simp_all only [Sum.elim_inl, PFun.mem_restrict, Finset.mem_coe]
+            | inr val_1 => simp_all only [Sum.elim_inr]
+          next h_1 => simp_all only [↓reduceDIte, Part.not_mem_none]
+        · intro a_1
+          unfold ArityToTuple at *
+          simp_all only [PFun.dom_mk, DatabaseInstance.validSchema_def]
+          split
+          next h_1 =>
+            simp_all only [↓reduceDIte]
+            have ⟨k, hk⟩ := Term.cases (tMap (RelationSchema.index h_1))
+            have z := Term.RealizeSome.fromRelMap (RelationSchema.index h_1) ht
+            rw [hk]
+            simp_all only [realize_var]
+            cases k with
+            | inl val =>
+              simp [Part.dom_iff_mem] at z a_1
+              simp [a_1, z]
+            | inr val_1 => simp_all only [Sum.elim_inr]
+          next h_1 => simp_all only [↓reduceDIte, Part.not_mem_none]
+      simp_all only [folStruc_apply_RelMap]
+
+
+@[simp]
+theorem Relmap.tuple_restrict2 [folStruc : folStruc dbi] {t : Tuple} (h : ↑((BoundedQuery.R dbi.schema rn tMap).schema) ⊆ t.Dom) :
+  folStruc.RelMap (fol.Rel dbi.schema rn) (fun i ↦ realize (Sum.elim t iv) (tMap i)) →
+    folStruc.RelMap (fol.Rel dbi.schema rn) (fun i ↦ realize (Sum.elim (PFun.restrict t h) iv) (tMap i)) := by
+      intro ht
+      have z : (ArityToTuple fun i ↦ realize (Sum.elim (t.restrict h) iv) (tMap i)) = (ArityToTuple fun i ↦ realize (Sum.elim t iv) (tMap i)) := by
+        ext a v
+        apply Iff.intro
+        · intro a_1
+          unfold ArityToTuple at *
+          simp_all only [PFun.dom_mk, DatabaseInstance.validSchema_def]
+          split
+          next h_1 =>
+            simp_all only [↓reduceDIte, Part.dom_iff_mem]
+            have ⟨k, hk⟩ := Term.cases (tMap (RelationSchema.index h_1))
+            rw [hk]
+            simp_all only [realize_var]
+            cases k with
+            | inl val => simp_all only [Sum.elim_inl, PFun.mem_restrict, Finset.mem_coe]
+            | inr val_1 => simp_all only [Sum.elim_inr]
+          next h_1 => simp_all only [↓reduceDIte, Part.not_mem_none]
+        · intro a_1
+          simp_all
+          have arityDom := RelationInstance.validSchema.def ht
+          unfold ArityToTuple at *
+          simp_all only [PFun.dom_mk, DatabaseInstance.validSchema_def]
+          split
+          next h_1 =>
+            simp_all only [↓reduceDIte]
+            have ⟨k, hk⟩ := Term.cases (tMap (RelationSchema.index h_1))
+            rw [hk]
+            simp_all only [realize_var]
+            cases k with
+            | inl
+              val =>
+              simp_all only [Sum.elim_inl, PFun.mem_restrict, BoundedQuery.schema.R_def, Set.coe_toFinset,
+                Set.mem_setOf_eq, and_true]
+              simp_all only [BoundedQuery.schema.R_def, Set.coe_toFinset]
+              use RelationSchema.index h_1
+              unfold varFinsetLeft
+              split
+              . simp_all only [var.injEq, Sum.inl.injEq, Finset.mem_singleton]
+              . simp_all only [var.injEq, reduceCtorEq]
+              . simp_all [emptyStructure]
+            | inr val_1 => simp_all only [Sum.elim_inr]
+          next h_1 => simp_all only [↓reduceDIte, Part.not_mem_none]
+      simp_all only [folStruc_apply_RelMap]
+
+
+@[simp]
+theorem BoundedQuery.Realize.tuple_restrict [folStruc dbi] {n : ℕ} {q : BoundedQuery n} {t : Tuple} {iv : Fin n →. Value} (h_wt : q.isWellTyped dbi.schema)
+  : q.Realize dbi t' iv → (h : t'.Dom ⊆ t.Dom) → t' = t.restrict h → q.Realize dbi t iv := by
+    intro a h a_1
+    induction q with
+    | R dbs rn tMap =>
+      simp_all only [realizeSome.def, toFormula_rel, BoundedFormula.realize_rel]
+      simp_all
+      subst h_wt
+      exact Relmap.tuple_restrict a h rfl
+
+    | tEq sq t₁ t₂ ih  =>
+      simp_all only [«def», isWellTyped.tEq_def, toFormula_tEq, BoundedFormula.realize_inf,
+        true_and, forall_const, implies_true]
+      obtain ⟨left, right⟩ := a
+
+      have hDom₁ := Realize.all_terms h_wt.1 left t₁ h_wt.2.1
+      have hDom₂ := Realize.all_terms h_wt.1 left t₂ h_wt.2.2
+
+      · simp_all [BoundedFormula.Realize]
+        obtain ⟨left_1, right_1⟩ := h_wt
+        obtain ⟨left_3, right_1⟩ := right_1
+        have ⟨t₁, ht₁⟩ := Term.cases t₁
+        have ⟨t₂, ht₂⟩ := Term.cases t₂
+        simp_all [ht₁, ht₂]
+        cases t₁ with
+        | inl att₁ =>
+          simp_all
+          cases t₂ with
+          | inl att₂ =>
+            by_cases hd₁ : (t' att₁).Dom
+            . by_cases hd₂ : (t' att₂).Dom
+              . simp [Part.ext_iff] at right ⊢
+                simp [Part.dom_iff_mem] at hd₁ hd₂
+                intro v
+                apply Iff.intro
+                . intro hv
+                  exact ((right v).mp (And.intro hd₁ hv)).2
+                . intro hv
+                  exact ((right v).mpr (And.intro hd₂ hv)).2
+              . simp_all
+            . simp_all
+          | inr fin₂ =>
+            by_cases (t' att₁).Dom
+            . simp_all
+              rw [← right]
+              ext v
+              simp [PFun.mem_restrict]
+              intro a
+              subst ht₁ ht₂
+              simp_all only
+              exact Part.dom_iff_mem.mp hDom₂
+            . simp_all
+        | inr fin₁ =>
+          cases t₂ with
+          | inl att₂ =>
+            by_cases (t' att₂).Dom
+            . simp_all
+              ext v
+              simp [PFun.mem_restrict]
+              intro a
+              subst ht₁ ht₂
+              simp_all only
+              exact Part.dom_iff_mem.mp hDom₂
+            . simp_all
+          | inr fin₂ =>
+            simp_all
+
+    | ex q ih =>
+      simp [BoundedQuery.Realize.def] at a ⊢ h_wt
+      have ⟨w, hw⟩ := a
+      use w
+      simp_all only [«def», forall_const]
+
+    | _ => simp_all [BoundedQuery.Realize.def]
+
+@[simp]
+theorem BoundedQuery.Realize.tuple_restrict2 [folStruc dbi] {n : ℕ} {q : BoundedQuery n} {t : Tuple} {iv : Fin n →. Value} (h_wt : q.isWellTyped dbi.schema)
+  : (h : ↑q.schema ⊆ t.Dom) → q.Realize dbi t iv → q.Realize dbi (t.restrict h) iv := by
+    intro h h_rel
+    induction q with
+    | R dbs rn tMap =>
+      simp_all only [isWellTyped.R_def, toFormula_rel, BoundedFormula.realize_rel]
+      subst h_wt
+      simp_all [Relmap.tuple_restrict2 h h_rel,BoundedQuery.Realize.def]
+
+
+    | tEq sq t₁ t₂ ih  =>
+      simp only [«def», isWellTyped.tEq_def, toFormula_tEq, BoundedFormula.realize_inf,
+        true_and, forall_const, implies_true, BoundedQuery.Realize.def] at h_rel h_wt ⊢
+      simp_all
+      obtain ⟨left, right⟩ := h_rel
+
+      have hDom₁ := Realize.all_terms h_wt.1 left t₁ h_wt.2.1
+      have hDom₂ := Realize.all_terms h_wt.1 left t₂ h_wt.2.2
+
+      have ⟨t₁, ht₁⟩ := Term.cases t₁
+      subst ht₁
+      have ⟨t₂, ht₂⟩ := Term.cases t₂
+      subst ht₂
+
+      simp_all only [«def», realize_var, true_and]
+      obtain ⟨left_1, right_1⟩ := h_wt
+      obtain ⟨left_2, right_1⟩ := right_1
+      cases t₁ with
+      | inl val =>
+        cases t₂ with
+        | inl val_1 =>
+          simp_all only [Sum.elim_inl, hasSafeTerm_mem_schema]
+          ext a : 1
+          simp_all only [Part.dom_iff_mem, BoundedFormula.Realize, realize_var, Sum.elim_inl,
+            schema, PFun.mem_restrict, Finset.mem_coe, true_and]
+        | inr val_2 =>
+          simp_all only [Sum.elim_inl, hasSafeTerm_mem_schema, Sum.elim_inr]
+          simp_all only [BoundedFormula.Realize, realize_var, Sum.elim_inl, Sum.elim_inr]
+          ext a : 1
+          simp_all only [PFun.mem_restrict, schema.tEq_def, Finset.mem_coe, true_and]
+      | inr val_1 =>
+        cases t₂ with
+        | inl val =>
+          simp_all only [Sum.elim_inr, Sum.elim_inl, hasSafeTerm_mem_schema]
+          ext a : 1
+          simp_all only [Part.dom_iff_mem, BoundedFormula.Realize, realize_var, Sum.elim_inr,
+            Sum.elim_inl, schema, PFun.mem_restrict, Finset.mem_coe, true_and]
+        | inr val_2 =>
+          simp_all only [Sum.elim_inr]
+          exact right
+
+    | and q₁ q₂ ih₁ ih₂ =>
+      simp only [«def», isWellTyped.and_def, toFormula_and, BoundedFormula.realize_inf,
+        forall_const, implies_true] at h_rel h_wt ⊢
+      simp_all
+      obtain ⟨left, right⟩ := h_wt
+      obtain ⟨left_1, right_1⟩ := h_rel
+      apply And.intro
+      · have h': ↑q₁.schema ⊆ t.Dom := by simp_all
+        have := ih₁ h' left_1
+        have h'' : ↑q₁.schema ⊆ ↑(q₁.and q₂).schema := by simp
+        exact tuple_restrict left (ih₁ h' left_1) h'' rfl
+      · have h': ↑q₂.schema ⊆ t.Dom := by simp_all
+        have := ih₂ h' right_1
+        have h'' : ↑q₂.schema ⊆ ↑(q₁.and q₂).schema := by simp
+        exact tuple_restrict right (ih₂ h' right_1) h'' rfl
+
+    | ex q ih =>
+      simp only [«def», toFormula_ex, BoundedFormula.realize_ex, Nat.succ_eq_add_one,
+        isWellTyped.ex_def] at h_rel h_wt ⊢
+      simp_all only [«def», forall_const]
+      obtain ⟨w, h_1⟩ := h_rel
+      apply Exists.intro
+      · apply @ih
+        simp_all only [schema.ex_def, forall_true_left]
+        apply h_1
